

# Yoneda lemma

Alyson Mei

January 9, 2026

## Conventions

- $\mathcal{C}$  – locally small category;
- $\lambda AB.\mathcal{C}(A, B) : \mathcal{C}^{\text{op}} \times \mathcal{C} \rightarrow \mathcal{C}$  – Hom functor;
  - For brevity, if the context is clear,  $A, B := \mathcal{C}(A, B)$ ;
  - $A, _ := \mathcal{C}(A, _) := \lambda B.\mathcal{C}(A, B) : \mathcal{C} \rightarrow \mathcal{Set}$ ; similarly for  $_ , B : \mathcal{C}^{\text{op}} \rightarrow \mathcal{Set}$ ;
- $F, G := [F, G]$  – class of natural transformations between  $F$  and  $G$ ;
- $\simeq$  denotes isomorphisms of objects,  $\cong$  emphasizes that isomorphism between objects extends to isomorphism between functors.

# 1 Yoneda lemma

**Theorem 1.1** (Yoneda lemma). For a given  $F : \mathcal{C} \rightarrow \mathcal{S}et$  (resp.  $F : \mathcal{C}^{op} \rightarrow \mathcal{S}et$ )

$$\lambda AF.\mathcal{C}(A, -), F \simeq \lambda AF.FA \text{ (resp. } \lambda AF.\mathcal{C}(-, A), F \simeq \lambda AF.FA) :$$

$$\begin{array}{ccc} \mathcal{C} \times \mathcal{S}et^{\mathcal{C}} & \begin{array}{c} \xrightarrow{\lambda AF.\mathcal{C}(A, -), F} \\ \Downarrow \simeq \\ \xrightarrow{\lambda AF.FA} \end{array} & \mathcal{S}et \\ & & \end{array} \quad \Bigg| \quad \begin{array}{ccc} \mathcal{C}^{op} \times \mathcal{S}et^{\mathcal{C}^{op}} & \begin{array}{c} \xrightarrow{\lambda AF.\mathcal{C}(-, A), F} \\ \Downarrow \simeq \\ \xrightarrow{\lambda AF.FA} \end{array} & \mathcal{S}et \end{array} .$$

**Proof** (Covariant option).

1.  $\eta : \mathcal{C}(A, -) \rightarrow F$  is uniquely determined by the choice of  $\eta_A(\text{id}_A) \in FA$  :

$$\begin{array}{ccccc} A & A, A & \xrightarrow{\eta_A} & FA & \text{id}_A \longmapsto \eta_A(\text{id}_A) \\ f \downarrow & f \circ - \downarrow & & \downarrow Ff & \downarrow \\ B & A, B & \xrightarrow{\eta_B} & FB & f \longmapsto \eta_B(f) = Ff(\eta_A(\text{id}_A)) \end{array} .$$

Note, that this is possible, because for all  $B : \text{obj}(\mathcal{C}) \cup_{f \in A, B} \text{im}(f \circ -) = A, B$ . So, we established a family of isomorphisms:

$$\Phi_{A, F} : \mathcal{C}(A, -), F \xrightarrow{\simeq} FA; \Phi^{-1} : x \mapsto \eta^x, \text{ where } \eta_A^x(\text{id}_A) = x.$$

2.  $\Phi$  extends to a natural transformation between  $\lambda AF.\mathcal{C}(A, -), F$  and  $\lambda AF.FA$  :

$$\begin{array}{ccccc} A & F & \mathcal{C}(A, -), F & \xrightarrow{\Phi_{A, F}} & F(A) \\ \downarrow \alpha_{\bullet} & \downarrow \beta & \downarrow \beta \circ - \circ (\lambda \varphi. \alpha_{\bullet} \circ \varphi) & & \downarrow F' \alpha_{\bullet} \circ \beta_A \\ A' & F' & \mathcal{C}(A', -), F' & \xrightarrow{\Phi_{A', F'}} & F'(A') \end{array}$$

$$\begin{array}{ccc} \eta^x & \longmapsto & x \\ \downarrow & & \downarrow \\ \eta^{x'} := \beta \circ \eta^x \circ (\lambda \varphi. \alpha_{\bullet} \circ \varphi) & \longmapsto & \Phi(\eta^{x'}) = F' \alpha_{\bullet} \circ \beta_A(x) \end{array} .$$

To prove the equality, we need to compare the  $x' = \eta^{x'}(\text{id}_{A'})$  and  $F' \alpha_{\bullet} \circ \beta_A(x)$ . It follows from the naturality conditions for  $\beta$  and  $\eta^x$ :

$$\begin{array}{ccccc} A & FA & \xrightarrow{\beta_A} & F'A & \text{id}_A : A, A \xrightarrow{\eta_A^x} \eta_{A'}^x(\text{id}_{A'}) = x : FA \\ \alpha_{\bullet} \downarrow & F \alpha_{\bullet} \downarrow & & \downarrow F' \alpha_{\bullet} & \downarrow F \alpha_{\bullet} \\ A' & FA' & \xrightarrow{\beta_{A'}} & F'A' & \alpha_{\bullet} : A, A' \xrightarrow{\eta_{A'}^x} \eta_{A'}^x(\alpha_{\bullet}) = F \alpha_{\bullet}(x) : FA' \end{array}$$

$$\beta_{A'} \circ \eta_{A'}^x \circ (\lambda \varphi. \alpha_{\bullet} \circ \varphi)(\text{id}_{A'}) = \beta_{A'} \circ \eta_{A'}^x(\alpha_{\bullet}) = \beta_{A'} \circ F \alpha_{\bullet}(x) = F' \alpha_{\bullet} \circ \beta_A(x).$$

## 2 Corollaries

**Definition 2.1** (Yoneda embedding).

$$Y := \lambda A. \mathcal{C}(A, -) : \mathcal{C}^{\text{op}} \rightarrow \mathcal{Set}^{\mathcal{C}}$$

$$\begin{array}{ccc} A & & B, - \\ \downarrow f & & \downarrow - \circ f \\ B & & A, - \end{array} .$$

**Proposition 2.2** (Fully faithfulness). Yoneda embedding is a fully faithful functor.

**Proof.** For an arbitrary  $B : \text{obj}(\mathcal{C})$ , in the covariant Yoneda lemma set  $F := \mathcal{C}(B, -)$ . This gives us a natural isomorphism:

$$\mathcal{C}(A, -), \mathcal{C}(B, -) \cong \mathcal{C}(B, A)$$

So, the mapping of morphisms under  $Y$  is bijective.

**Corollary 2.3** (Small rephrasings).

1. Every natural transformation between Hom functors from  $\mathcal{Set}^{\mathcal{C}}$  is given by a unique corresponding arrow between objects in  $\mathcal{C}$ ;
2.  $A \simeq B \Leftrightarrow \mathcal{C}(A, -) \simeq \mathcal{C}(B, -)$  (note that functors preserve isomorphisms).